src/proofs/no_slashable_attestations/supporting_lemmas/dv_next_invs_1_7.dfy
@@ -42,7 +42,7 @@ module DV_Next_Invs_1_7
     ensures inv_only_dv_construct_signed_attestation_signature(dv')
     { }    
 
-    lemma lemma_inv4_dv_next_helper(
+    lemma lemma_inv_queued_att_duty_is_dvn_seq_of_att_duty_dv_next_helper(
         dv: DVState,
         event: DV.Event,
         dv': DVState
@@ -50,15 +50,15 @@ module DV_Next_Invs_1_7
     requires inv_quorum_constraints(dv)    
     requires NextEventPreCond(dv, event)
     requires NextEvent(dv, event, dv')  
-    requires inv4(dv)    
+    requires inv_queued_att_duty_is_dvn_seq_of_att_duty(dv)    
     requires event.HonestNodeTakingStep?
     requires dv.honest_nodes_states[event.node].all_rcvd_duties == dv'.honest_nodes_states[event.node].all_rcvd_duties
-    ensures inv4(dv')
+    ensures inv_queued_att_duty_is_dvn_seq_of_att_duty(dv')
     {
 
     }    
 
-    lemma lemma_inv4_dv_next(
+    lemma lemma_inv_queued_att_duty_is_dvn_seq_of_att_duty_dv_next(
         dv: DVState,
         event: DV.Event,
         dv': DVState
@@ -66,8 +66,8 @@ module DV_Next_Invs_1_7
     requires inv_quorum_constraints(dv)    
     requires NextEventPreCond(dv, event)
     requires NextEvent(dv, event, dv')  
-    requires inv4(dv)
-    ensures inv4(dv')
+    requires inv_queued_att_duty_is_dvn_seq_of_att_duty(dv)
+    ensures inv_queued_att_duty_is_dvn_seq_of_att_duty(dv')
     {        
         match event 
         {
@@ -80,7 +80,7 @@ module DV_Next_Invs_1_7
                         assert dv'.index_next_attestation_duty_to_be_served 
                                     == dv.index_next_attestation_duty_to_be_served + 1;
                         forall hn | hn in dv.honest_nodes_states.Keys  
-                        ensures inv4_body(hn, dv'.honest_nodes_states[hn].all_rcvd_duties, dv'.sequence_attestation_duties_to_be_served, dv'.index_next_attestation_duty_to_be_served);                                                         
+                        ensures inv_queued_att_duty_is_dvn_seq_of_att_duty_body(hn, dv'.honest_nodes_states[hn].all_rcvd_duties, dv'.sequence_attestation_duties_to_be_served, dv'.index_next_attestation_duty_to_be_served);                                                         
                         {
                             if hn != node 
                             {
@@ -102,13 +102,13 @@ module DV_Next_Invs_1_7
                                            && dv'.sequence_attestation_duties_to_be_served[k].node == hn
                                            && dv'.sequence_attestation_duties_to_be_served[k].attestation_duty == duty;
                                 }
-                                assert inv4_body(hn, dv'.honest_nodes_states[hn].all_rcvd_duties, dv'.sequence_attestation_duties_to_be_served, dv'.index_next_attestation_duty_to_be_served);
+                                assert inv_queued_att_duty_is_dvn_seq_of_att_duty_body(hn, dv'.honest_nodes_states[hn].all_rcvd_duties, dv'.sequence_attestation_duties_to_be_served, dv'.index_next_attestation_duty_to_be_served);
                             }
                             else 
                             {                                   
                                 var curr_index := dv.index_next_attestation_duty_to_be_served;
                                 var new_duty := dv.sequence_attestation_duties_to_be_served[curr_index].attestation_duty;
-                                lemma_inv4_f_serve_attestation_duty(dvc, new_duty, dvc');    
+                                lemma_inv_queued_att_duty_is_dvn_seq_of_att_duty_f_serve_attestation_duty(dvc, new_duty, dvc');    
                                 var new_duty_set := {new_duty};
                                 assert dvc'.all_rcvd_duties == dvc.all_rcvd_duties + new_duty_set;                                                            
                                 // assert new_duty in dvc'.all_rcvd_duties;                                                          
@@ -139,35 +139,35 @@ module DV_Next_Invs_1_7
                                     }
                                 }     
 
-                                assert inv4_body(hn, dv'.honest_nodes_states[hn].all_rcvd_duties, dv'.sequence_attestation_duties_to_be_served, dv'.index_next_attestation_duty_to_be_served); 
+                                assert inv_queued_att_duty_is_dvn_seq_of_att_duty_body(hn, dv'.honest_nodes_states[hn].all_rcvd_duties, dv'.sequence_attestation_duties_to_be_served, dv'.index_next_attestation_duty_to_be_served); 
                                                    
                             }
                         }     
-                        assert inv4(dv');                   
+                        assert inv_queued_att_duty_is_dvn_seq_of_att_duty(dv');                   
                         
                     case AttConsensusDecided(id, decided_attestation_data) => 
-                        lemma_inv4_f_att_consensus_decided(dvc, id, decided_attestation_data, dvc');    
-                        assert inv4(dv');                   
+                        lemma_inv_queued_att_duty_is_dvn_seq_of_att_duty_f_att_consensus_decided(dvc, id, decided_attestation_data, dvc');    
+                        assert inv_queued_att_duty_is_dvn_seq_of_att_duty(dv');                   
                         
                     case ReceivedAttestationShare(attestation_share) =>                          
-                        lemma_inv4_f_listen_for_attestation_shares(dvc, attestation_share, dvc');  
-                        lemma_inv4_dv_next_helper(dv, event, dv');                   
+                        lemma_inv_queued_att_duty_is_dvn_seq_of_att_duty_f_listen_for_attestation_shares(dvc, attestation_share, dvc');  
+                        lemma_inv_queued_att_duty_is_dvn_seq_of_att_duty_dv_next_helper(dv, event, dv');                   
    
                     case ImportedNewBlock(block) => 
                         var dvc := add_block_to_bn(dvc, nodeEvent.block);
-                        lemma_inv4_f_listen_for_new_imported_blocks(dvc, block, dvc');    
-                        assert inv4(dv');                    
+                        lemma_inv_queued_att_duty_is_dvn_seq_of_att_duty_f_listen_for_new_imported_blocks(dvc, block, dvc');    
+                        assert inv_queued_att_duty_is_dvn_seq_of_att_duty(dv');                    
                                                 
                     case ResendAttestationShares => 
-                        assert inv4(dv');                        
+                        assert inv_queued_att_duty_is_dvn_seq_of_att_duty(dv');                        
                         
                     case NoEvent => 
-                        assert inv4(dv');
+                        assert inv_queued_att_duty_is_dvn_seq_of_att_duty(dv');
                         
                 }
 
             case AdeversaryTakingStep(node, new_attestation_share_sent, messagesReceivedByTheNode) =>
-                assert inv4(dv');
+                assert inv_queued_att_duty_is_dvn_seq_of_att_duty(dv');
                 
         }        
     }   
