src/proofs/no_slashable_attestations/supporting_lemmas/proofs_intermediate_steps.dfy
@@ -77,7 +77,7 @@ module Proofs_Intermediate_Steps
         dv: DVState
     )    
     requires inv_quorum_constraints(dv)  
-    requires inv4(dv)
+    requires inv_queued_att_duty_is_dvn_seq_of_att_duty(dv)
     requires inv_is_sequence_attestation_duties_to_be_serves_orders(dv)
     ensures concl_future_att_duty_is_higher_than_rcvd_att_duty(dv)    
     {   
@@ -90,7 +90,7 @@ module Proofs_Intermediate_Steps
         {
             var dvc := dv.honest_nodes_states[hn];
 
-            assert inv4_body( hn, dvc.all_rcvd_duties, 
+            assert inv_queued_att_duty_is_dvn_seq_of_att_duty_body( hn, dvc.all_rcvd_duties, 
                               dv.sequence_attestation_duties_to_be_served, 
                               dv.index_next_attestation_duty_to_be_served);
 
@@ -117,7 +117,7 @@ module Proofs_Intermediate_Steps
         dv: DVState
     )    
     requires inv_quorum_constraints(dv)  
-    requires inv4(dv)
+    requires inv_queued_att_duty_is_dvn_seq_of_att_duty(dv)
     requires inv_queued_att_duty_is_rcvd_duty(dv)
     requires inv_is_sequence_attestation_duties_to_be_serves_orders(dv)
     requires concl_future_att_duty_is_higher_than_rcvd_att_duty(dv)
@@ -132,7 +132,7 @@ module Proofs_Intermediate_Steps
         {
             var dvc := dv.honest_nodes_states[hn];
 
-            assert inv4_body(hn, dvc.all_rcvd_duties,
+            assert inv_queued_att_duty_is_dvn_seq_of_att_duty_body(hn, dvc.all_rcvd_duties,
                              dv.sequence_attestation_duties_to_be_served,
                              dv.index_next_attestation_duty_to_be_served);
             assert inv_queued_att_duty_is_rcvd_duty_body(dvc);
